Current status

kremlib/kremstr.h
@@ -18,4 +18,8 @@ static inline uint32_t bufstrcpy(char *dst, const char *src) {
   return end - dst;
 }
 
+static inline uint32_t print_u32(char *dst, uint32_t i) {
+  return sprintf(dst, "%"PRIu32, i);
+}
+
 #endif
